---
id: "1092"
title: "Shortest Common Supersequence "
companyTags: "Unknown"
slug: "shortest-common-supersequence"
difficulty: "Hard"
tags: ["String", "Dynamic Programming"]
---

### Explanation
To find the shortest common supersequence of two strings, we can use dynamic programming. Let `dp[i][j]` represent the length of the shortest common supersequence of `str1[0...i-1]` and `str2[0...j-1]`. We can build this table by considering the following cases:
- If the characters at the current positions are equal, then the current character is part of the supersequence. So, `dp[i][j] = dp[i-1][j-1] + 1`.
- If the characters are different, we have two options: either include `str1[i-1]` in the supersequence or `str2[j-1]`. So, `dp[i][j] = min(dp[i-1][j], dp[i][j-1]) + 1`.

Finally, to reconstruct the shortest common supersequence, we can start from `dp[m][n]` and backtrack by considering the characters and transitions made during the dp table construction.

```java
class Solution {
    public String shortestCommonSupersequence(String str1, String str2) {
        int m = str1.length();
        int n = str2.length();
        int[][] dp = new int[m+1][n+1];

        for (int i = 1; i <= m; i++) {
            dp[i][0] = i;
        }
        for (int j = 1; j <= n; j++) {
            dp[0][j] = j;
        }

        for (int i = 1; i <= m; i++) {
            for (int j = 1; j <= n; j++) {
                if (str1.charAt(i-1) == str2.charAt(j-1)) {
                    dp[i][j] = dp[i-1][j-1] + 1;
                } else {
                    dp[i][j] = Math.min(dp[i-1][j], dp[i][j-1]) + 1;
                }
            }
        }

        StringBuilder sb = new StringBuilder();
        int i = m, j = n;
        while (i > 0 && j > 0) {
            if (str1.charAt(i-1) == str2.charAt(j-1)) {
                sb.insert(0, str1.charAt(i-1));
                i--;
                j--;
            } else if (dp[i-1][j] < dp[i][j-1]) {
                sb.insert(0, str1.charAt(i-1));
                i--;
            } else {
                sb.insert(0, str2.charAt(j-1));
                j--;
            }
        }

        while (i > 0) {
            sb.insert(0, str1.charAt(i-1));
            i--;
        }
        while (j > 0) {
            sb.insert(0, str2.charAt(j-1));
            j--;
        }

        return sb.toString();
    }
}
```

#### C++
```cpp
class Solution {
public:
    string shortestCommonSupersequence(string str1, string str2) {
        int m = str1.length();
        int n = str2.length();
        vector<vector<int>> dp(m+1, vector<int>(n+1, 0));

        for (int i = 1; i <= m; i++) {
            dp[i][0] = i;
        }
        for (int j = 1; j <= n; j++) {
            dp[0][j] = j;
        }

        for (int i = 1; i <= m; i++) {
            for (int j = 1; j <= n; j++) {
                if (str1[i-1] == str2[j-1]) {
                    dp[i][j] = dp[i-1][j-1] + 1;
                } else {
                    dp[i][j] = min(dp[i-1][j], dp[i][j-1]) + 1;
                }
            }
        }

        string result = "";
        int i = m, j = n;
        while (i > 0 && j > 0) {
            if (str1[i-1] == str2[j-1]) {
                result = str1[i-1] + result;
                i--;
                j--;
            } else if (dp[i-1][j] < dp[i][j-1]) {
                result = str1[i-1] + result;
                i--;
            } else {
                result = str2[j-1] + result;
                j--;
            }
        }

        while (i > 0) {
            result = str1[i-1] + result;
            i--;
        }
        while (j > 0) {
            result = str2[j-1] + result;
            j--;
        }

        return result;
    }
};
```

#### Python
```python
class Solution:
    def shortestCommonSupersequence(self, str1: str, str2: str) -> str:
        m, n = len(str1), len(str2)
        dp = [[0] * (n+1) for _ in range(m+1)]

        for i in range(1, m+1):
            dp[i][0] = i
        for j in range(1, n+1):
            dp[0][j] = j

        for i in range(1, m+1):
            for j in range(1, n+1):
                if str1[i-1] == str2[j-1]:
                    dp[i][j] = dp[i-1][j-1] + 1
                else:
                    dp[i][j] = min(dp[i-1][j], dp[i][j-1]) + 1

        result = ""
        i, j = m, n
        while i > 0 and j > 0:
            if str1[i-1] == str2[j-1]:
                result = str1[i-1] + result
                i -= 1
                j -= 1
            elif dp[i-1][j] < dp[i][j-1]:
                result = str1[i-1] + result
                i -= 1
            else:
                result = str2[j-1] + result
                j -= 1

        while i > 0:
            result = str1[i-1] + result
            i -= 1
        while j > 0:
            result = str2[j-1] + result
            j -= 1

        return result
```