---
id: "1143"
title: "Longest Common Subsequence"
companyTags: "Unknown"
slug: "longest-common-subsequence"
difficulty: "Medium"
tags: ["String", "Dynamic Programming"]
---

### Explanation
To solve this problem, we can use dynamic programming. We will create a 2D array to store the length of the longest common subsequence up to each point in the two strings. We will iterate over the strings and fill in the array based on certain conditions. At the end, the value in the bottom right corner of the array will represent the length of the longest common subsequence.

Here are the steps:
1. Create a 2D array `dp` of size `(text1.length()+1) x (text2.length()+1)`.
2. Initialize the first row and first column of the array with zeros.
3. Iterate over the strings `text1` and `text2`.
4. If the characters at the current indices are the same, update `dp[i][j] = dp[i-1][j-1] + 1`.
5. Otherwise, update `dp[i][j] = max(dp[i-1][j], dp[i][j-1])`.
6. The value at `dp[text1.length()][text2.length()]` will be the length of the longest common subsequence.

The time complexity of this approach is O(m*n), where m and n are the lengths of the input strings. The space complexity is also O(m*n) since we are using a 2D array to store intermediate results.
```java
class Solution {
    public int longestCommonSubsequence(String text1, String text2) {
        int m = text1.length();
        int n = text2.length();
        int[][] dp = new int[m+1][n+1];
        
        for (int i = 1; i <= m; i++) {
            for (int j = 1; j <= n; j++) {
                if (text1.charAt(i-1) == text2.charAt(j-1)) {
                    dp[i][j] = dp[i-1][j-1] + 1;
                } else {
                    dp[i][j] = Math.max(dp[i-1][j], dp[i][j-1]);
                }
            }
        }
        
        return dp[m][n];
    }
}
```

```cpp
class Solution {
public:
    int longestCommonSubsequence(string text1, string text2) {
        int m = text1.length();
        int n = text2.length();
        vector<vector<int>> dp(m+1, vector<int>(n+1, 0));
        
        for (int i = 1; i <= m; i++) {
            for (int j = 1; j <= n; j++) {
                if (text1[i-1] == text2[j-1]) {
                    dp[i][j] = dp[i-1][j-1] + 1;
                } else {
                    dp[i][j] = max(dp[i-1][j], dp[i][j-1]);
                }
            }
        }
        
        return dp[m][n];
    }
};
```

```python
class Solution:
    def longestCommonSubsequence(self, text1: str, text2: str) -> int:
        m, n = len(text1), len(text2)
        dp = [[0] * (n+1) for _ in range(m+1)]
        
        for i in range(1, m+1):
            for j in range(1, n+1):
                if text1[i-1] == text2[j-1]:
                    dp[i][j] = dp[i-1][j-1] + 1
                else:
                    dp[i][j] = max(dp[i-1][j], dp[i][j-1])
        
        return dp[m][n]
```