---
id: "1171"
title: "Remove Zero Sum Consecutive Nodes from Linked List"
companyTags: "Unknown"
slug: "remove-zero-sum-consecutive-nodes-from-linked-list"
difficulty: "Medium"
tags: ["Hash Table", "Linked List"]
---

## Explanation

To solve this problem, we can use a hashmap to keep track of the running sum of the linked list nodes encountered so far. If we encounter the same running sum again, it means that the nodes between the two occurrences of the sum have a sum of 0. We can then remove those nodes from the linked list.

We iterate through the linked list, keeping track of the running sum and the node at which we first encountered that running sum. If we encounter the same running sum again, we remove all nodes between the two occurrences from the linked list. 

We also need to handle the case where the running sum is 0 (i.e., the accumulated sum from the beginning of the list is 0). In this case, we remove all nodes up to the current node.

After processing the entire linked list, we return the head of the modified linked list.

Time complexity: O(n) where n is the number of nodes in the linked list.
Space complexity: O(n) for the hashmap.
```java
class Solution {
    public ListNode removeZeroSumSublists(ListNode head) {
        ListNode dummy = new ListNode(0);
        dummy.next = head;
        
        Map<Integer, ListNode> map = new HashMap<>();
        
        int sum = 0;
        for (ListNode curr = dummy; curr != null; curr = curr.next) {
            sum += curr.val;
            map.put(sum, curr);
        }
        
        sum = 0;
        for (ListNode curr = dummy; curr != null; curr = curr.next) {
            sum += curr.val;
            curr.next = map.get(sum).next;
        }
        
        return dummy.next;
    }
}
```

```cpp
class Solution {
public:
    ListNode* removeZeroSumSublists(ListNode* head) {
        ListNode* dummy = new ListNode(0);
        dummy->next = head;
        
        unordered_map<int, ListNode*> map;
        
        int sum = 0;
        for (ListNode* curr = dummy; curr != nullptr; curr = curr->next) {
            sum += curr->val;
            map[sum] = curr;
        }
        
        sum = 0;
        for (ListNode* curr = dummy; curr != nullptr; curr = curr->next) {
            sum += curr->val;
            curr->next = map[sum]->next;
        }
        
        return dummy->next;
    }
};
```

```python
class Solution:
    def removeZeroSumSublists(self, head: ListNode) -> ListNode:
        dummy = ListNode(0)
        dummy.next = head
        
        sums = {}
        sum_val = 0
        current = dummy
        
        while current:
            sum_val += current.val
            if sum_val in sums:
                current = sums[sum_val].next
                temp = sum_val + current.val
                while temp != sum_val:
                    del sums[temp]
                    current = current.next
                    temp += current.val
                sums[sum_val].next = current.next
            else:
                sums[sum_val] = current
            current = current.next
        
        return dummy.next
```