---
id: "88"
title: "Merge Sorted Array"
companyTags: "Unknown"
slug: "merge-sorted-array"
difficulty: "Easy"
tags: ["Array", "Two Pointers", "Sorting"]
---

## Explanation
To merge two sorted arrays *nums1* and *nums2* into *nums1* in-place, we can start from the end of both arrays and compare elements. By placing the larger element at the end of *nums1*, we can ensure that the merged array remains sorted. This approach allows us to merge the two arrays in-place without using any extra space.

- Time complexity: O(m + n) where m is the number of elements in *nums1* and n is the number of elements in *nums2*.
- Space complexity: O(1) as we are merging the arrays in-place.
```java
class Solution {
    public void merge(int[] nums1, int m, int[] nums2, int n) {
        int i = m - 1;
        int j = n - 1;
        int k = m + n - 1;

        while (i >= 0 && j >= 0) {
            if (nums1[i] > nums2[j]) {
                nums1[k--] = nums1[i--];
            } else {
                nums1[k--] = nums2[j--];
            }
        }

        while (j >= 0) {
            nums1[k--] = nums2[j--];
        }
    }
}
```

### C++
```cpp
class Solution {
public:
    void merge(vector<int>& nums1, int m, vector<int>& nums2, int n) {
        int i = m - 1;
        int j = n - 1;
        int k = m + n - 1;

        while (i >= 0 && j >= 0) {
            if (nums1[i] > nums2[j]) {
                nums1[k--] = nums1[i--];
            } else {
                nums1[k--] = nums2[j--];
            }
        }

        while (j >= 0) {
            nums1[k--] = nums2[j--];
        }
    }
};
```

### Python
```python
class Solution:
    def merge(self, nums1: List[int], m: int, nums2: List[int], n: int) -> None:
        i = m - 1
        j = n - 1
        k = m + n - 1
        
        while i >= 0 and j >= 0:
            if nums1[i] > nums2[j]:
                nums1[k] = nums1[i]
                i -= 1
            else:
                nums1[k] = nums2[j]
                j -= 1
            k -= 1
        
        while j >= 0:
            nums1[k] = nums2[j]
            j -= 1
            k -= 1
```